began creating an readme for artifact eval

theories/Ref/Example.v
@@ -20,47 +20,25 @@ Import MonadNotation.
 Local Open Scope monad_scope.
 Local Open Scope list_scope.
 
-Definition halve_specm {Γ : call_stack} {E} `{EncodedType E} 
-           (l : list nat) : SpecM E Γ (list nat * list nat) :=
-  MrecS (list nat) (fun _ => list nat * list nat)%type
-         (fun l => 
-           match l with
-           | nil => ret (nil, nil)
-           | x :: nil => ret (x :: nil, nil)
-           | x :: y :: t => '(l1,l2) <- CallS t;;
-                         ret (x :: l1, y :: l2) end
-        ) l.
 
-Definition merge_specm {Γ : call_stack} {E} `{EncodedType E} 
-           (l1 l2 : list nat) : SpecM E Γ (list nat) :=
-  MrecS (list nat * list nat) (fun _ => list nat)
-        (fun '(l1, l2) => 
-           match (l1, l2) with
-           | (nil, _) => ret l2
-           | (_, nil) => ret l1
-           | (x :: tx, y :: ty) =>
-               if Nat.leb x y
-               then
-                 l <- CallS (tx, y :: ty);;
-                 ret (x :: l)
-               else
-                 l <- CallS (x :: tx, ty);;
-                 ret (y :: l)
-                end
+Variant evenoddE : Type:=
+  | even (n : nat) : evenoddE
+  | odd  (n : nat) : evenoddE.
+Instance EncodingType_evenoddE : EncodingType evenoddE := fun _ => bool.
 
-        ) (l1,l2).
+Variant voidE : Type :=.
 
-Definition sort_specm {Γ : call_stack} {E} `{EncodedType E} 
-           (l : list nat) : SpecM E Γ (list nat) :=
-  MrecS (list nat) (fun _ => list nat)
-        (fun l => 
-           match l with
-           | nil => ret nil
-           | x :: nil => ret (x :: nil)
-           | _ => '(l1,l2) <- halve_specm l;;
-                 l1s <- CallS l1;;
-                 l2s <- CallS l2;;
-                 merge_specm l1s l2s 
-           end
-        ) l.
-(* a closed program is parametric in its call stack *)
+Instance EncodingType_voidE : EncodingType voidE := fun _ => False.
+
+Definition evenodd_body : forall eo : evenoddE, (entree (evenoddE + voidE)) (encodes eo) :=
+  fun eo =>
+    match eo with
+    | even n => if Nat.eqb n 0
+               then Ret true
+               else trigger (odd (n - 1))
+    | odd  n => if Nat.eqb n 0
+               then Ret false
+               else trigger (even (n - 1))
+    end.
+Definition evenodd : evenoddE -> entree voidE bool :=
+  mrec evenodd_body.
