Artifact_README.md
@@ -1,0 +1,56 @@
+# Core ITree Specifications Library
+## Definitions Table
+- `paper_name` -> `repo_name` at `filpath:line#`
+    - Notes
+- `server_impl` -> `server_impl` at `theories/Rel/SortEx.v:600`
+- `server_spec` -> `server_spec` at `theories/Rel/SortEx.v:608`
+- `EncodingType` -> `EncodingType` at `theories/Basics/HeterogeneousRelations.v:13`
+    - While in the paper, the `EncodingType` class requires a function named `response_type`, in the code it is called `encodes`
+- `ReSum` -> `ReSum` at `theories/Core/SubEvent.v:18` and `theories/Core/SubEvent.v:19`
+    - While in the paper, `ReSum` is presented as a single typeclass requiring two functions, in the code it is presented as two typeclasses each requiring one function
+- `trigger` -> `trigger` at `theories/Core/SubEvent.v:30`
+- `itree` -> `entree` at `theories/Core/EnTreeDefinition.v:9-21`
+    - The paper presents `itree` with a positive type coinductive definition, while the code repository uses negative types. This causes minor differences in many definitions related to ITrees
+- `spin` -> `spin` at `theories/Core/EnTreeDefinition.v:77`
+- `euttF` -> `eqitF` at `theories/Eq/Eqit.v:37`
+    - `eqitF` is more general than `euttF`, containing boolean parameters that control whether inductive `Tau` steps can be made, as well as the `vclo` parameter which can be useful for certain interactions with the `paco` library, but to understand this code you can assume it is always set to the identity function and can be ignored
+- `eutt` -> `eutt` at `theories/Eq/Eqit.v:78`
+    - While `eutt` is defined on line `78`, the application of the `paco` libraries greatest fixpoint combinator occurs on line `74`
+- `bind` -> `bind` at `theories/Core/EnTreeDefinition.v:46-61`
+    - In the code, `bind` is defined in terms of `subst`, which performs an identical computation with the continuation and the tree swapped
+- `interp_mrec` -> `interp_mrec` at `theories/Ref/MRecSpec.v:26-37`
+- `mrec` -> `mrec` at `theories/Ref/MRecSpec.v:38`
+- `evenodd` -> `evenodd` at `theories/Ref/Example.v:24-44`
+- `Rel` -> `Rel` at `theories/Basics/HeterogeneousRelations.v:20`
+- `PostRel` -> `PostRel` at `theories/Basics/HeterogeneousRelations.v:21`
+- `RComposePostRel` -> `RComposePostRel` at `theories/Basics/HeterogeneousRelations.v:31`
+- `CoveredType` -> `QuantType` at `theories/Basics/QuantType.v:33`
+- `forall_spec` -> `forall_spec` at `theories/Ref/EnTreeSpecDefinition.v:99`
+- `exists_spec` -> `exists_spec` at `theories/Ref/EnTreeSpecDefinition.v:101`
+- `assume_spec` -> `assume_spec` at `theories/Ref/EnTreeSpecDefinition.v:104`
+- `assert_spec` -> `assert_spec` at `theories/Ref/EnTreeSpecDefinition.v:107`
+- `SpecEvent` -> `SpecEvent` at `theories/Ref/EnTreeSpecDefinition.v:26`
+- `itree_spec` -> `entree_spec` at `theories/Ref/EnTreeSpecDefinition.v:51`
+- `refinesF` -> `refinesF` at `theories/Ref/EnTreeSpecDefinition.v:65`
+- `refines` -> `refines` at `theories/Ref/EnTreeSpecDefinition.v:95`
+- `padded_refines` -> `padded_refines` at `theories/Ref/EnTreeSpecFacts.v:838`
+- `interp_mrec_spec` -> `interp_mrec_spec` at `theories/Ref/MRecSpec.v:43-55`
+- `mrec_spec` -> `mrec_spec` at `theories/Ref/MRecSpec.v:56`
+- TODO concrete
+- `rec_fix_spec` -> `rec_fix_spec` at `theories/Ref/RecSpecFix.v:50`
+-  `total_spec` -> `total_spec'` at `theories/Ref/RecFixSpecTotal.v:43`
+- `total_spec_fix` -> `total_spec_fix` at `theories/Ref/RecFixSpecTotal.v:53`
+- `merge` -> `merge` at `theories/Ref/SortEx.v:241`
+- `merge_pre` -> `merge_pre` at `theories/Ref/SortEx.v:261` 
+- `merge_post` -> `merge_post` at `theories/Ref/SortEx.v:264`
+- `rdec_merge` -> `rdec_merge` at `theories/Ref/SortEx.v:107`
+## Theorems
+- `padded_refines_bind` -> `padded_refines_bind` at `theories/Ref/EnTreeSpecCombinatorFacts.v:110`
+- `padded_refines_trans` -> `padded_refines_trans` at `theories/Ref/EnTreeSpecFacts/v:872`
+- `padded_refines_mrec` -> `padded_refine_mrec` at `theories/Ref/EnTreeSpecCombinatorFacts.v:423`
+- `total_spec_fix_correct` -> `total_spec_fix_refines_total_spec'` at `theories/Ref/RecFixSpecTotal.v:66`
+- `merge_correct` -> `merge_correct` at `theories/Ref/SortEx.v:423`
+- `server_correct` -> `server_correct` at `theories/Ref/RecFixSpecTotal.v:619`
+# Heapster Tool
+
+# MBox Example
